src/hog/tree_set.lean
@@ -73,6 +73,7 @@ inductive stree (α : Type) [linear_order α] : ∀ {low high : bounded α}, low
 | node : ∀ {low high} (x : α) {q : low < element x} {r : element x < high}
            (left : stree q) (right : stree r), stree (lt_trans q r)
 
+
 example: stree ℕ (by { trivial } : bottom < top) :=
   stree.node 20 
     (stree.empty true.intro)
@@ -157,11 +158,16 @@ end
 
 @[reducible]
 def stree.forall {α : Type} [linear_order α] (p : α → Prop) [decidable_pred p] :
-  ∀ {low high : bounded α} {b : low < high} (t : stree α b) , bool
+  ∀ {low high : bounded α} {b : low < high} (t : stree α b), bool
 | _ _ _ (stree.empty _) := tt
 | _ _ _ (stree.leaf x _ _):= decidable.to_bool (p x)
 | _ _ _ (stree.node x left right) := 
   decidable.to_bool (p x) && stree.forall left && stree.forall right
+
+def stree.option_forall {α : Type} [linear_order α] (p : α → Prop) [decidable_pred p] :
+  ∀ {low high : bounded α} {b : low < high} (t : option (stree α b)), bool
+| _ _ _ none := ff
+| _ _ _ (some t) := stree.forall p t
 
 lemma stree.forall_is_forall {α : Type} [linear_order α] (p : α → Prop) [decidable_pred p]:
   ∀ {low high : bounded α} {b : low < high} (t : stree α b), 
@@ -236,7 +242,6 @@ def tset.option_mem {α : Type} [linear_order α] (x : α) : option (tset α) �
 | none := ff
 | (some t) := tset.mem x t
 
-
 instance tset.has_mem {α : Type} [linear_order α]: has_mem α (tset α) :=
   { mem := λ x t, tset.mem x t }
 
@@ -252,110 +257,6 @@ lemma tset.forall_is_forall {α : Type} [linear_order α] (p : α → Prop) [dec
   ∀ (t : tset α), stree.forall p t = tt → ∀ (x : α), x ∈ t → p x :=
   by apply stree.forall_is_forall
 
-def tset.intersection {α : Type} [linear_order α] : tset α → tset α → tset α := sorry
-
--- The type of edges
-structure Edge : Type :=
-  (edge : lex ℕ ℕ)
-  (src_lt_trg : edge.fst < edge.snd . obviously)
-
-instance Edge_linear_order : linear_order Edge :=
-  linear_order.lift (λ (u : Edge), u.edge) (λ u v H, begin cases u, cases v, simp, assumption end)
-
-inductive smap (α β: Type) [linear_order α] : ∀ {low high : bounded α}, low < high → Type
-| empty : ∀ {low high} (p : low < high), smap p
-| leaf : ∀ {low high} (key : α) (val : β) (lowx : low < element key) (xhigh : element key < high), smap (lt_trans lowx xhigh)
-| node : ∀ {low high} (key : α) (val : β) {q : low < element key} {r : element key < high}
-           (left : smap q) (right : smap r), smap (lt_trans q r)
-
-example : smap ℕ ℕ (by { trivial } : bottom < top) :=
-  smap.node 1 10
-    (smap.leaf 0 666 (by trivial) (by obviously))
-    (smap.leaf 2 20 (by obviously) (by trivial))
-
-@[reducible]
-def smap.contains_key {α β: Type} [linear_order α] (key : α) :
-    ∀ {low high : bounded α} {p : low < high}, smap α β p → bool
-| low high p (smap.empty _) := ff
-| low high p (smap.leaf x _ _ _) := (key = x)
-| low high p (smap.node x _ left right) :=
-    decidable.lt_by_cases key x
-      (λ _, smap.contains_key left)
-      (λ _, tt)
-      (λ _, smap.contains_key right)
-
-
-@[reducible]
-def smap.contains_val {α β: Type} [linear_order α] [decidable_eq β] (val : β) :
-    ∀ {low high : bounded α} {p : low < high}, smap α β p → bool
-| low high p (smap.empty _) := ff
-| low high p (smap.leaf _ x _ _) := (val = x)
-| low high p (smap.node _ x left right) := (val = x) || smap.contains_val left || smap.contains_val right
-
-@[reducible]
-def smap.val_at {α β : Type} [linear_order α] (key: α) :
-    ∀ {low high : bounded α} {p : low < high}, smap α β p → option β
-| low high p (smap.empty _) := none
-| low high p (smap.leaf x val _ _) :=     
-    decidable.lt_by_cases key x
-      (λ _, none)
-      (λ _, some val)
-      (λ _, none)
-| low high p (smap.node x val left right) :=     
-    decidable.lt_by_cases key x
-      (λ _, smap.val_at left)
-      (λ _, some val)
-      (λ _, smap.val_at right)
-
-def smap.size {α β: Type} [linear_order α] : ∀ {low high : bounded α} {p : low < high}, smap α β p → ℕ
-| low high p (smap.empty _) := 0
-| low high p (smap.leaf x _ _ _) := 1
-| low high p (smap.node x _ left right) := 1 + smap.size left + smap.size right
-
-def smap.to_map {α β : Type} [linear_order α] :
-  ∀ {low high : bounded α} {p : low < high}, 
-  smap α β p → (α → option β) 
-:=
-λ low high p t x, smap.val_at x t
-
-@[reducible]
-def smap.forall {α β : Type} [linear_order α] (p : β → Prop) [decidable_pred p] :
-  ∀ {low high : bounded α} {b : low < high} (t : smap α β b) , bool
-| _ _ _ (smap.empty _) := tt
-| _ _ _ (smap.leaf _ val _ _):= decidable.to_bool (p val)
-| _ _ _ (smap.node _ val left right) := 
-  decidable.to_bool (p val) && smap.forall left && smap.forall right
-
-@[reducible]
-def extend_prop {β : Type} (p : β → Prop) : option β → Prop
-| none := false
-| (some b) := p b
-
-
-lemma smap.forall_is_forall {α β : Type} [linear_order α] (p : β → Prop) [decidable_pred p]:
-  ∀ {low high : bounded α} {b : low < high} (t : smap α β b), 
-  smap.forall p t = tt → ∀ (x : α), smap.contains_key x t → (extend_prop p) (smap.val_at x t) :=  
-begin
-  intros low high b t,
-  induction t with _ _ _ _ _ _ _ _ _ _  _ y B ,
-  { simp },
-  { simp [smap.forall, smap.val_at, decidable.lt_by_cases] },
-  { simp [smap.forall, smap.val_at], intros py lall rall x,
-    apply (decidable.lt_by_cases x y),
-    { intro xy, simp [ smap.contains_key, decidable.lt_by_cases, xy], obviously }, -- can we find a better proof that obviously?
-    { intro xy, simp [ smap.contains_key, decidable.lt_by_cases, xy], assumption },
-    { intro yx, simp [ smap.contains_key, decidable.lt_by_cases, yx, lt_asymm yx], tautology },
-  }
-end
-
-def tmap (α β : Type) [lo : linear_order α] := @smap α β lo bottom top true.intro
-
-def tmap.contains_key {α β : Type} [linear_order α] (key : α) : tmap α β → bool := smap.contains_key key
-
-def tmap.contains_val {α β : Type} [linear_order α] [decidable_eq β] (val : β) : tmap α β → bool := smap.contains_val val
-
-def tmap.val_at {α β : Type} [linear_order α] (key : α) : tmap α β → option β := smap.val_at key
-
-def tmap.to_map {α β : Type} [linear_order α] : tmap α β → (α → option β) := smap.to_map
+-- def tset.intersection {α : Type} [linear_order α] : tset α → tset α → tset α := sorry
 
 end tree_set
