src/hog/tree_map.lean
@@ -1,0 +1,125 @@
+import .tree_set
+
+namespace tree_map
+
+open tree_set
+open tree_set.bounded
+
+inductive smap (α β: Type) [linear_order α] : ∀ {low high : bounded α}, low < high → Type
+| empty : ∀ {low high} (p : low < high), smap p
+| leaf : ∀ {low high} (key : α) (val : β) (lowx : low < element key) (xhigh : element key < high), smap (lt_trans lowx xhigh)
+| node : ∀ {low high} (key : α) (val : β) {q : low < element key} {r : element key < high}
+           (left : smap q) (right : smap r), smap (lt_trans q r)
+
+example : smap ℕ ℕ (by { trivial } : bottom < top) :=
+  smap.node 1 10
+    (smap.leaf 0 666 (by trivial) (by obviously))
+    (smap.leaf 2 20 (by obviously) (by trivial))
+
+@[reducible]
+def smap.contains_key {α β: Type} [linear_order α] (key : α) :
+    ∀ {low high : bounded α} {p : low < high}, smap α β p → bool
+| low high p (smap.empty _) := ff
+| low high p (smap.leaf x _ _ _) := (key = x)
+| low high p (smap.node x _ left right) :=
+    decidable.lt_by_cases key x
+      (λ _, smap.contains_key left)
+      (λ _, tt)
+      (λ _, smap.contains_key right)
+
+
+@[reducible]
+def smap.contains_val {α β: Type} [linear_order α] [decidable_eq β] (val : β) :
+    ∀ {low high : bounded α} {p : low < high}, smap α β p → bool
+| low high p (smap.empty _) := ff
+| low high p (smap.leaf _ x _ _) := (val = x)
+| low high p (smap.node _ x left right) := (val = x) || smap.contains_val left || smap.contains_val right
+
+@[reducible]
+def smap.val_at {α β : Type} [linear_order α] (key: α) :
+    ∀ {low high : bounded α} {p : low < high}, smap α β p → option β
+| low high p (smap.empty _) := none
+| low high p (smap.leaf x val _ _) :=     
+    decidable.lt_by_cases key x
+      (λ _, none)
+      (λ _, some val)
+      (λ _, none)
+| low high p (smap.node x val left right) :=     
+    decidable.lt_by_cases key x
+      (λ _, smap.val_at left)
+      (λ _, some val)
+      (λ _, smap.val_at right)
+
+def smap.size {α β: Type} [linear_order α] : ∀ {low high : bounded α} {p : low < high}, smap α β p → ℕ
+| low high p (smap.empty _) := 0
+| low high p (smap.leaf x _ _ _) := 1
+| low high p (smap.node x _ left right) := 1 + smap.size left + smap.size right
+
+def smap.to_map {α β : Type} [linear_order α] :
+  ∀ {low high : bounded α} {p : low < high}, 
+  smap α β p → (α → option β) 
+:=
+λ low high p t x, smap.val_at x t
+
+@[reducible]
+def smap.forall_keys {α β : Type} [linear_order α] (p : α → Prop) [decidable_pred p] :
+  ∀ {low high : bounded α} {b : low < high} (t : smap α β b) , bool
+| _ _ _ (smap.empty _) := tt
+| _ _ _ (smap.leaf key _ _ _):= decidable.to_bool (p key)
+| _ _ _ (smap.node key _ left right) := 
+  decidable.to_bool (p key) && smap.forall_keys left && smap.forall_keys right
+
+
+@[reducible]
+def smap.forall {α β : Type} [linear_order α] (p : α × β → Prop) [decidable_pred p] :
+  ∀ {low high : bounded α} {b : low < high} (t : smap α β b) , bool
+| _ _ _ (smap.empty _) := tt
+| _ _ _ (smap.leaf key val _ _):= decidable.to_bool (p (key, val))
+| _ _ _ (smap.node key val left right) := 
+  decidable.to_bool (p (key, val)) && smap.forall left && smap.forall right
+
+@[reducible]
+def extend_prop {β : Type} (p : β → Prop) : option β → Prop
+| none := false
+| (some b) := p b
+
+@[reducible]
+def option_prod {α β : Type} : option α → option β → option (α × β)
+| none none := none
+| (some a) none := none
+| none (some b) := none
+| (some a) (some b) := some (a, b)
+
+@[reducible]
+def option_prod_curried {α β : Type} : option α × option β → option (α × β) := λ ⟨ a, b ⟩, option_prod a b
+
+lemma smap.forall_is_forall {α β : Type} [linear_order α] (p : α × β → Prop) [decidable_pred p]:
+  ∀ {low high : bounded α} {b : low < high} (t : smap α β b), 
+  smap.forall p t = tt 
+  → ∀ (x : α), smap.contains_key x t 
+  → (extend_prop p) (option_prod_curried (some x, (smap.val_at x t))) :=
+begin
+  intros low high b t,
+  induction t with _ _ _ _ _ _ _ _ _ _  _ y B ,
+  { simp },
+  { simp [smap.forall, smap.val_at, decidable.lt_by_cases, option_prod, option_prod_curried] },
+  { simp [smap.forall, smap.val_at], intros py lall rall x,
+    apply (decidable.lt_by_cases x y),
+    { intro xy, simp [ smap.contains_key, decidable.lt_by_cases, xy], obviously }, -- can we find a better proof that obviously?
+    { intro xy, simp [ smap.contains_key, decidable.lt_by_cases, xy], assumption },
+    { intro yx, simp [ smap.contains_key, decidable.lt_by_cases, yx, lt_asymm yx], tautology },
+  }
+end
+
+def tmap (α β : Type) [lo : linear_order α] := @smap α β lo bottom top true.intro
+
+def tmap.contains_key {α β : Type} [linear_order α] (key : α) : tmap α β → bool := smap.contains_key key
+
+def tmap.contains_val {α β : Type} [linear_order α] [decidable_eq β] (val : β) : tmap α β → bool := smap.contains_val val
+
+def tmap.val_at {α β : Type} [linear_order α] (key : α) : tmap α β → option β := smap.val_at key
+
+def tmap.to_map {α β : Type} [linear_order α] : tmap α β → (α → option β) := smap.to_map
+
+
+end tree_map
